fstar/treekem/code/MLS.TreeKEM.API.fst
@@ -1,31 +1,38 @@
 module MLS.TreeKEM.API
 
 open Comparse
-open MLS.Result
 open MLS.Crypto
 open MLS.NetworkTypes
 open MLS.Tree
-open MLS.TreeCommon
-open MLS.TreeCommon.Lemmas
-open MLS.TreeKEM.Types
-open MLS.TreeKEM.Operations
-open MLS.TreeKEM.Invariants
-open MLS.TreeKEM.Invariants.Proofs
 open MLS.NetworkBinder.Properties
+open MLS.TreeKEM.Types
+open MLS.TreeKEM.Invariants
+open MLS.TreeKEM.API.KeySchedule.Types
+//open MLS.TreeKEM.API.KeySchedule
+open MLS.TreeKEM.API.Tree.Types
+//open MLS.TreeKEM.API.Tree
 open MLS.TreeKEM.API.Types
+open MLS.Result
+
+module T = MLS.TreeKEM.API.Tree
+module KS = MLS.TreeKEM.API.KeySchedule
+
+#set-options "--fuel 0 --ifuel 0"
 
 (*** Create ***)
 
 val create:
   #bytes:Type0 -> {|crypto_bytes bytes|} ->
   hpke_private_key bytes -> bytes ->
-  treekem_state bytes 0
-let create #bytes #cb dec_key enc_key =
-  {
-    levels = 0;
-    tree = TLeaf (Some ({public_key = enc_key} <: treekem_leaf bytes));
-    priv = PLeaf dec_key
-  }
+  bytes ->
+  result (treekem_state bytes 0 & bytes)
+let create #bytes #cb dec_key enc_key epoch_secret =
+  let tree_state = T.create dec_key enc_key in
+  let? (keyschedule_state, encryption_secret) = KS.create epoch_secret in
+  return ({
+    tree_state;
+    keyschedule_state;
+  }, encryption_secret)
 
 (*** Welcome ***)
 
@@ -33,27 +40,15 @@ val welcome:
   #bytes:Type0 -> {|crypto_bytes bytes|} ->
   #l:nat ->
   t:treekem bytes l 0{treekem_invariant t} -> hpke_private_key bytes -> option (bytes & nat) -> leaf_ind:nat{leaf_ind < pow2 l /\ Some? (leaf_at t leaf_ind)} ->
-  result (treekem_state bytes leaf_ind)
-let welcome #bytes #cb #l t leaf_decryption_key opt_path_secret_and_inviter_ind leaf_ind =
-  let priv = create_empty_priv leaf_decryption_key in
-  let? priv =
-    match opt_path_secret_and_inviter_ind with
-    | None -> return priv
-    | Some (path_secret, inviter_ind) ->
-      if not (leaf_ind <> inviter_ind) then
-        error "welcome: leaf_index and inviter index are the same"
-      else if not (inviter_ind < pow2 l) then
-        error "welcome: inviter_index too big"
-      else
-        let path_secret_level = compute_least_common_ancestor_level priv inviter_ind in
-        let? (priv, _) = path_apply_path t priv path_secret path_secret_level in
-        return priv
-  in
-  return {
-    levels = l;
-    tree = t;
-    priv;
-  }
+  bytes ->
+  result (treekem_state bytes leaf_ind & bytes)
+let welcome #bytes #cb #l t leaf_decryption_key opt_path_secret_and_inviter_ind leaf_ind epoch_secret =
+  let? tree_state = T.welcome t leaf_decryption_key opt_path_secret_and_inviter_ind leaf_ind in
+  let? (keyschedule_state, encryption_secret) = KS.create epoch_secret in
+  return ({
+    tree_state;
+    keyschedule_state;
+  }, encryption_secret)
 
 (*** Add ***)
 
@@ -62,28 +57,8 @@ val add:
   treekem_state bytes leaf_ind -> treekem_leaf bytes ->
   treekem_state bytes leaf_ind & nat
 let add #bytes #cb #leaf_ind st kp =
-  match find_empty_leaf st.tree with
-  | Some i -> (
-    treekem_invariant_add st.tree i kp;
-    treekem_priv_invariant_add st.tree st.priv i kp;
-    ({ st with
-      tree = tree_add st.tree i kp;
-    }, (i <: nat))
-  )
-  | None -> (
-    find_empty_leaf_tree_extend st.tree;
-    let extended_tree = tree_extend st.tree in
-    let i = Some?.v (find_empty_leaf extended_tree) in
-    treekem_invariant_extend st.tree;
-    treekem_priv_invariant_extend st.tree st.priv;
-    treekem_invariant_add extended_tree i kp;
-    treekem_priv_invariant_add extended_tree (path_extend st.priv) i kp;
-    ({ st with
-      levels = st.levels+1;
-      tree = tree_add extended_tree i kp;
-      priv = path_extend st.priv;
-    }, (i <: nat))
-  )
+  let (tree_state, i) = T.add st.tree_state kp in
+  ({ st with tree_state }, i)
 
 (*** Update ***)
 
@@ -92,138 +67,122 @@ val update:
   st:treekem_state bytes leaf_ind -> treekem_leaf bytes -> treekem_index st ->
   treekem_state bytes leaf_ind
 let update #bytes #cb #leaf_ind st lp i =
-  treekem_invariant_update st.tree i lp;
-  treekem_priv_invariant_update st.tree st.priv i lp;
-  { st with tree = tree_update st.tree i lp; }
+  { st with tree_state = T.update st.tree_state lp i }
 
 (*** Remove ***)
-
-val fully_truncate:
-  #bytes:Type0 -> {|crypto_bytes bytes|} -> #leaf_ind:nat ->
-  st:treekem_state bytes leaf_ind ->
-  Tot (treekem_state bytes leaf_ind)
-  (decreases st.levels)
-let rec fully_truncate #bytes #cb #leaf_ind st =
-  if 1 <= st.levels && is_tree_empty (TNode?.right st.tree) then (
-    if leaf_ind >= pow2 (st.levels-1) then (
-      MLS.TreeCommon.Lemmas.is_tree_empty_leaf_at (TNode?.right st.tree) leaf_ind;
-      false_elim ()
-    ) else (
-      treekem_invariant_truncate st.tree;
-      treekem_priv_invariant_truncate st.tree st.priv;
-      fully_truncate {
-        levels = st.levels-1;
-        tree = tree_truncate st.tree;
-        priv = path_truncate st.priv;
-      }
-    )
-  ) else (
-    st
-  )
 
 val remove:
   #bytes:Type0 -> {|crypto_bytes bytes|} -> #leaf_ind:nat ->
   st:treekem_state bytes leaf_ind -> i:treekem_index st{i <> leaf_ind} ->
   treekem_state bytes leaf_ind
 let remove #bytes #cb #leaf_ind st i =
-  treekem_invariant_remove st.tree i;
-  treekem_priv_invariant_remove st.tree st.priv i;
-  fully_truncate { st with
-    tree = tree_remove st.tree i;
-  }
+  { st with tree_state = T.remove st.tree_state i }
 
 (*** Process Commit ***)
 
+type full_commit_args (#bytes:Type0) {|crypto_bytes bytes|} (#leaf_ind:nat) (st:treekem_tree_state bytes leaf_ind) = {
+  commit_leaf_ind: commit_leaf_ind:MLS.TreeKEM.API.Tree.Types.treekem_index st{commit_leaf_ind <> leaf_ind};
+  path: path:pathkem bytes st.levels 0 commit_leaf_ind{path_filtering_ok st.tree path};
+  excluded_leaves: excluded_leaves:list nat{~(List.Tot.memP leaf_ind excluded_leaves)};
+}
+
 val commit:
   #bytes:Type0 -> {|crypto_bytes bytes|} -> #leaf_ind:nat ->
-  st:treekem_state bytes leaf_ind -> #li:treekem_index st{li <> leaf_ind} -> p:pathkem bytes st.levels 0 li{path_filtering_ok st.tree p} -> excluded_leaves:list nat{~(List.Tot.memP leaf_ind excluded_leaves)} -> group_context_nt bytes ->
+  st:treekem_state bytes leaf_ind -> option (full_commit_args st.tree_state) -> option bytes -> group_context_nt bytes -> group_context_nt bytes ->
   result (treekem_state bytes leaf_ind & bytes)
-let commit #bytes #cb #leaf_ind st #li p excluded_leaves group_context =
-  let un_added_tree = un_add st.tree excluded_leaves in
-  treekem_invariant_un_add st.tree excluded_leaves;
-  treekem_priv_invariant_un_add st.tree st.priv excluded_leaves;
-  if not (check_update_path_ciphertexts_lengthes un_added_tree p) then (
-    error "TreeKEM.commit: bad UpdatePath ciphertext lengths"
-  ) else (
-    weaken_path_filtering_ok st.tree p;
-    path_filtering_weak_ok_un_add st.tree p excluded_leaves;
-    let? (path_secret, least_common_ancestor_level) = get_path_secret un_added_tree st.priv p group_context in
-    let new_tree = tree_apply_path st.tree p in
-    let? (new_priv, root_secret) = path_apply_path new_tree st.priv path_secret least_common_ancestor_level in
-    treekem_invariant_apply_path st.tree p;
-    treekem_priv_invariant_apply_path st.tree st.priv p path_secret least_common_ancestor_level;
-    return ({ st with
-      tree = new_tree;
-      priv = new_priv;
-    }, root_secret)
-  )
+let commit #bytes #cb #leaf_ind st opt_full_commit_args opt_psk provisional_group_context new_group_context =
+  let? (tree_state, opt_commit_secret) =
+    match opt_full_commit_args with
+    | None -> return (st.tree_state, None)
+    | Some args ->
+      let? (new_tree_state, commit_secret) = T.commit st.tree_state args.path args.excluded_leaves provisional_group_context in
+      return (new_tree_state, Some commit_secret)
+  in
+  let? (keyschedule_state, encryption_secret, _) = KS.commit st.keyschedule_state opt_commit_secret opt_psk new_group_context in
+  return ({
+    tree_state;
+    keyschedule_state;
+  }, encryption_secret)
 
 (*** Create Commit ***)
 
 val prepare_create_commit_entropy_lengths:
-  #bytes:Type0 -> {|crypto_bytes bytes|} ->
+  bytes:Type0 -> {|crypto_bytes bytes|} ->
   list nat
-let prepare_create_commit_entropy_lengths #bytes #cb =
-  [hpke_private_key_length #bytes; kdf_length #bytes]
+let prepare_create_commit_entropy_lengths bytes #cb =
+  T.prepare_create_commit_entropy_lengths bytes
 
 type pending_commit (#bytes:Type0) {|crypto_bytes bytes|} (#leaf_ind:nat) (st:treekem_state bytes leaf_ind) = {
-  path_secrets: path_secrets:path_secrets bytes st.levels 0 leaf_ind{path_filtering_ok st.tree path_secrets /\ forget_path_secrets path_secrets == generate_forgotten_path_secrets st.tree leaf_ind};
-  commit_secret: bytes;
+  pend: MLS.TreeKEM.API.Tree.pending_commit st.tree_state;
 }
 
 val prepare_create_commit:
   #bytes:Type0 -> {|crypto_bytes bytes|} -> #leaf_ind:nat ->
   st:treekem_state bytes leaf_ind ->
-  randomness bytes (prepare_create_commit_entropy_lengths #bytes) ->
-  result (pending_commit st & pre_pathkem bytes st.levels 0 leaf_ind)
+  randomness bytes (prepare_create_commit_entropy_lengths bytes) ->
+  result (pending_commit st & pre_pathkem bytes st.tree_state.levels 0 leaf_ind)
 let prepare_create_commit #bytes #cb #leaf_ind st rand =
-  let leaf_sk, rand = dest_randomness rand in
-  let path_secret_0, rand = dest_randomness rand in
-  let? (path_secrets, commit_secret) = generate_path_secrets st.tree leaf_sk path_secret_0 leaf_ind in
-  let? pre_upd_path = path_secrets_to_pre_pathkem path_secrets in
-  path_filtering_ok_generate_path_secrets st.tree leaf_sk path_secret_0 leaf_ind;
-  return ({
-    path_secrets;
-    commit_secret;
-  }, pre_upd_path)
+  let? (pend, path) = T.prepare_create_commit st.tree_state rand in
+  return ({pend}, path)
 
-val finalize_create_commit_entropy_lengths:
+val continue_create_commit_entropy_lengths:
   #bytes:Type0 -> {|crypto_bytes bytes|} -> #leaf_ind:nat ->
   st:treekem_state bytes leaf_ind -> list nat ->
   list nat
-let finalize_create_commit_entropy_lengths #bytes #cb #leaf_ind st added_leaves =
-  treekem_invariant_un_add st.tree added_leaves;
-  let path_secrets = generate_forgotten_path_secrets st.tree leaf_ind in
-  encrypt_path_secrets_entropy_lengths (un_add st.tree added_leaves) path_secrets
+let continue_create_commit_entropy_lengths #bytes #cb #leaf_ind st added_leaves =
+  T.finalize_create_commit_entropy_lengths st.tree_state added_leaves
 
-type create_commit_result (#bytes:Type0) {|crypto_bytes bytes|} (#leaf_ind:nat) (st:treekem_state bytes leaf_ind) = {
+type pending_commit_2 (bytes:Type0) {|crypto_bytes bytes|} (leaf_ind:nat) = {
   new_state: treekem_state bytes leaf_ind;
-  update_path: update_path:pathkem bytes st.levels 0 leaf_ind{path_filtering_ok st.tree update_path};
   commit_secret: bytes;
+}
+
+type continue_create_commit_result (#bytes:Type0) {|crypto_bytes bytes|} (#leaf_ind:nat) (st:treekem_state bytes leaf_ind) = {
+  update_path: update_path:pathkem bytes st.tree_state.levels 0 leaf_ind{path_filtering_ok st.tree_state.tree update_path};
   added_leaves_path_secrets: list bytes;
 }
 
-val finalize_create_commit:
+val continue_create_commit:
   #bytes:Type0 -> {|crypto_bytes bytes|} -> #leaf_ind:nat ->
   #st:treekem_state bytes leaf_ind ->
   pending_commit st ->
   added_leaves:list nat -> group_context_nt bytes ->
-  randomness bytes (finalize_create_commit_entropy_lengths st added_leaves) ->
-  result (create_commit_result st)
-let finalize_create_commit #bytes #cb #leaf_ind #st pending added_leaves group_context randomness =
-  treekem_invariant_un_add st.tree added_leaves;
-  let? (update_path, new_priv) = encrypt_path_secrets (un_add st.tree added_leaves) pending.path_secrets group_context randomness in
-  let? added_leaves_path_secrets = get_path_secret_of_added_leaves pending.path_secrets added_leaves in
-  let new_tree = tree_apply_path st.tree update_path in
-  path_filtering_ok_encrypt_path_secrets st.tree (un_add st.tree added_leaves) pending.path_secrets group_context randomness;
-  treekem_invariant_apply_path st.tree update_path;
-  treekem_priv_invariant_encrypt_path_secrets st.tree (un_add st.tree added_leaves) pending.path_secrets group_context randomness;
+  randomness bytes (continue_create_commit_entropy_lengths st added_leaves) ->
+  result (pending_commit_2 bytes leaf_ind & continue_create_commit_result st)
+let continue_create_commit #bytes #cb #leaf_ind #st pending added_leaves provisional_group_context randomness =
+  let? tree_commit_result = T.finalize_create_commit #bytes pending.pend added_leaves provisional_group_context randomness in
+  let new_state = { st with
+    tree_state = tree_commit_result.new_state;
+  } in
   return ({
-    new_state = { st with
-      tree = new_tree;
-      priv = new_priv;
-    };
-    update_path;
-    commit_secret = pending.commit_secret;
-    added_leaves_path_secrets;
+    new_state;
+    commit_secret = tree_commit_result.commit_secret;
+  }, {
+    update_path = tree_commit_result.update_path;
+    added_leaves_path_secrets = tree_commit_result.added_leaves_path_secrets;
   })
+
+type create_commit_result (bytes:Type0) {|crypto_bytes bytes|} (leaf_ind: nat) = {
+  new_state: treekem_state bytes leaf_ind;
+  encryption_secret: bytes;
+  // secrets needed to generate welcomes
+  welcome_secret: bytes;
+  joiner_secret: bytes;
+}
+
+val finalize_create_commit:
+  #bytes:Type0 -> {|crypto_bytes bytes|} -> #leaf_ind:nat ->
+  pending_commit_2 bytes leaf_ind  ->
+  group_context_nt bytes -> option bytes ->
+  result (create_commit_result bytes leaf_ind)
+let finalize_create_commit #bytes #cb #leaf_ind pending new_group_context opt_psk =
+  let? (keyschedule_state, encryption_secret, additional_secrets) = KS.commit pending.new_state.keyschedule_state (Some pending.commit_secret) opt_psk new_group_context in
+  return {
+    new_state = {
+      pending.new_state with
+      keyschedule_state;
+    };
+    encryption_secret;
+    welcome_secret = additional_secrets.welcome_secret;
+    joiner_secret = additional_secrets.joiner_secret;
+  }
