fstar/treekem/code/MLS.TreeKEM.API.KeySchedule.Types.fst
@@ -1,0 +1,20 @@
+module MLS.TreeKEM.API.KeySchedule.Types
+
+// All the keys that are not forward-secret within an epoch.
+// In particular, encryption_secret is not in this set of keys:
+// it is returned by the commit function
+
+type epoch_keys (bytes:Type0) = {
+  sender_data_secret: bytes;
+  exporter_secret: bytes;
+  external_secret: bytes;
+  confirmation_key: bytes;
+  membership_key: bytes;
+  resumption_psk: bytes;
+  epoch_authenticator: bytes;
+}
+
+type treekem_keyschedule_state (bytes:Type0) = {
+  epoch_keys: epoch_keys bytes;
+  init_secret: bytes;
+}
