fstar/treekem/code/MLS.TreeKEM.API.KeySchedule.fst
@@ -1,0 +1,57 @@
+module MLS.TreeKEM.API.KeySchedule
+
+open Comparse
+open MLS.Crypto
+open MLS.NetworkTypes
+open MLS.TreeKEM.API.KeySchedule.Types
+open MLS.TreeKEM.KeySchedule
+open MLS.Result
+
+val create:
+  #bytes:Type0 -> {|crypto_bytes bytes|} ->
+  bytes ->
+  result (treekem_keyschedule_state bytes & bytes)
+let create #bytes #cb epoch_secret =
+  let? sender_data_secret = secret_epoch_to_sender_data epoch_secret in
+  let? encryption_secret = secret_epoch_to_encryption epoch_secret in
+  let? exporter_secret = secret_epoch_to_exporter epoch_secret in
+  let? external_secret = secret_epoch_to_external epoch_secret in
+  let? confirmation_key = secret_epoch_to_confirmation epoch_secret in
+  let? membership_key = secret_epoch_to_membership epoch_secret in
+  let? resumption_psk = secret_epoch_to_resumption epoch_secret in
+  let? epoch_authenticator = secret_epoch_to_authentication epoch_secret in
+  let? init_secret = secret_epoch_to_init epoch_secret in
+  return (({
+    epoch_keys = {
+      sender_data_secret;
+      exporter_secret;
+      external_secret;
+      confirmation_key;
+      membership_key;
+      resumption_psk;
+      epoch_authenticator;
+    };
+    init_secret;
+  } <: treekem_keyschedule_state bytes), (encryption_secret <: bytes))
+
+type secrets_for_welcome (bytes:Type0) = {
+  joiner_secret: bytes;
+  welcome_secret: bytes;
+}
+
+val commit:
+  #bytes:Type0 -> {|crypto_bytes bytes|} ->
+  treekem_keyschedule_state bytes ->
+  option bytes ->
+  option bytes ->
+  group_context_nt bytes ->
+  result (treekem_keyschedule_state bytes & bytes & secrets_for_welcome bytes)
+let commit #bytes #cb st opt_commit_secret opt_psk new_group_context =
+  let? joiner_secret: bytes = secret_init_to_joiner st.init_secret opt_commit_secret (serialize _ new_group_context) in
+  let? epoch_secret: bytes = secret_joiner_to_epoch joiner_secret opt_psk (serialize _ new_group_context) in
+  let? welcome_secret: bytes = secret_joiner_to_welcome joiner_secret opt_psk in
+  let? (new_st, encryption_secret) = create epoch_secret in
+  return (new_st, encryption_secret, {
+    joiner_secret;
+    welcome_secret;
+  })
