fstar/treekem/code/MLS.TreeKEM.API.Tree.Types.fst
@@ -1,0 +1,14 @@
+module MLS.TreeKEM.API.Tree.Types
+
+open Comparse
+open MLS.Crypto
+open MLS.Tree
+open MLS.TreeKEM.Types
+
+type treekem_tree_state (bytes:Type0) {|crypto_bytes bytes|} (leaf_ind:nat) = {
+  levels: levels:nat{leaf_ind < pow2 levels};
+  tree: tree:treekem bytes levels 0{MLS.TreeKEM.Invariants.treekem_invariant tree};
+  priv: priv:treekem_priv bytes levels 0 leaf_ind{MLS.TreeKEM.Invariants.treekem_priv_invariant tree priv};
+}
+
+type treekem_index (#bytes:Type0) {|crypto_bytes bytes|} (#leaf_ind:nat) (st:treekem_tree_state bytes leaf_ind) = i:nat{i < pow2 st.levels}
