fstar/treekem/code/MLS.TreeKEM.API.Tree.fst
@@ -1,0 +1,229 @@
+module MLS.TreeKEM.API.Tree
+
+open Comparse
+open MLS.Result
+open MLS.Crypto
+open MLS.NetworkTypes
+open MLS.Tree
+open MLS.TreeCommon
+open MLS.TreeCommon.Lemmas
+open MLS.TreeKEM.Types
+open MLS.TreeKEM.Operations
+open MLS.TreeKEM.Invariants
+open MLS.TreeKEM.Invariants.Proofs
+open MLS.NetworkBinder.Properties
+open MLS.TreeKEM.API.Tree.Types
+
+(*** Create ***)
+
+val create:
+  #bytes:Type0 -> {|crypto_bytes bytes|} ->
+  hpke_private_key bytes -> bytes ->
+  treekem_tree_state bytes 0
+let create #bytes #cb dec_key enc_key =
+  {
+    levels = 0;
+    tree = TLeaf (Some ({public_key = enc_key} <: treekem_leaf bytes));
+    priv = PLeaf dec_key
+  }
+
+(*** Welcome ***)
+
+val welcome:
+  #bytes:Type0 -> {|crypto_bytes bytes|} ->
+  #l:nat ->
+  t:treekem bytes l 0{treekem_invariant t} -> hpke_private_key bytes -> option (bytes & nat) -> leaf_ind:nat{leaf_ind < pow2 l /\ Some? (leaf_at t leaf_ind)} ->
+  result (treekem_tree_state bytes leaf_ind)
+let welcome #bytes #cb #l t leaf_decryption_key opt_path_secret_and_inviter_ind leaf_ind =
+  let priv = create_empty_priv leaf_decryption_key in
+  let? priv =
+    match opt_path_secret_and_inviter_ind with
+    | None -> return priv
+    | Some (path_secret, inviter_ind) ->
+      if not (leaf_ind <> inviter_ind) then
+        error "welcome: leaf_index and inviter index are the same"
+      else if not (inviter_ind < pow2 l) then
+        error "welcome: inviter_index too big"
+      else
+        let path_secret_level = compute_least_common_ancestor_level priv inviter_ind in
+        let? (priv, _) = path_apply_path t priv path_secret path_secret_level in
+        return priv
+  in
+  return {
+    levels = l;
+    tree = t;
+    priv;
+  }
+
+(*** Add ***)
+
+val add:
+  #bytes:Type0 -> {|crypto_bytes bytes|} -> #leaf_ind:nat ->
+  treekem_tree_state bytes leaf_ind -> treekem_leaf bytes ->
+  treekem_tree_state bytes leaf_ind & nat
+let add #bytes #cb #leaf_ind st kp =
+  match find_empty_leaf st.tree with
+  | Some i -> (
+    treekem_invariant_add st.tree i kp;
+    treekem_priv_invariant_add st.tree st.priv i kp;
+    ({ st with
+      tree = tree_add st.tree i kp;
+    }, (i <: nat))
+  )
+  | None -> (
+    find_empty_leaf_tree_extend st.tree;
+    let extended_tree = tree_extend st.tree in
+    let i = Some?.v (find_empty_leaf extended_tree) in
+    treekem_invariant_extend st.tree;
+    treekem_priv_invariant_extend st.tree st.priv;
+    treekem_invariant_add extended_tree i kp;
+    treekem_priv_invariant_add extended_tree (path_extend st.priv) i kp;
+    ({ st with
+      levels = st.levels+1;
+      tree = tree_add extended_tree i kp;
+      priv = path_extend st.priv;
+    }, (i <: nat))
+  )
+
+(*** Update ***)
+
+val update:
+  #bytes:Type0 -> {|crypto_bytes bytes|} -> #leaf_ind:nat ->
+  st:treekem_tree_state bytes leaf_ind -> treekem_leaf bytes -> treekem_index st ->
+  treekem_tree_state bytes leaf_ind
+let update #bytes #cb #leaf_ind st lp i =
+  treekem_invariant_update st.tree i lp;
+  treekem_priv_invariant_update st.tree st.priv i lp;
+  { st with tree = tree_update st.tree i lp; }
+
+(*** Remove ***)
+
+val fully_truncate:
+  #bytes:Type0 -> {|crypto_bytes bytes|} -> #leaf_ind:nat ->
+  st:treekem_tree_state bytes leaf_ind ->
+  Tot (treekem_tree_state bytes leaf_ind)
+  (decreases st.levels)
+let rec fully_truncate #bytes #cb #leaf_ind st =
+  if 1 <= st.levels && is_tree_empty (TNode?.right st.tree) then (
+    if leaf_ind >= pow2 (st.levels-1) then (
+      MLS.TreeCommon.Lemmas.is_tree_empty_leaf_at (TNode?.right st.tree) leaf_ind;
+      false_elim ()
+    ) else (
+      treekem_invariant_truncate st.tree;
+      treekem_priv_invariant_truncate st.tree st.priv;
+      fully_truncate {
+        levels = st.levels-1;
+        tree = tree_truncate st.tree;
+        priv = path_truncate st.priv;
+      }
+    )
+  ) else (
+    st
+  )
+
+val remove:
+  #bytes:Type0 -> {|crypto_bytes bytes|} -> #leaf_ind:nat ->
+  st:treekem_tree_state bytes leaf_ind -> i:treekem_index st{i <> leaf_ind} ->
+  treekem_tree_state bytes leaf_ind
+let remove #bytes #cb #leaf_ind st i =
+  treekem_invariant_remove st.tree i;
+  treekem_priv_invariant_remove st.tree st.priv i;
+  fully_truncate { st with
+    tree = tree_remove st.tree i;
+  }
+
+(*** Process Commit ***)
+
+val commit:
+  #bytes:Type0 -> {|crypto_bytes bytes|} -> #leaf_ind:nat ->
+  st:treekem_tree_state bytes leaf_ind -> #li:treekem_index st{li <> leaf_ind} -> p:pathkem bytes st.levels 0 li{path_filtering_ok st.tree p} -> excluded_leaves:list nat{~(List.Tot.memP leaf_ind excluded_leaves)} -> group_context_nt bytes ->
+  result (treekem_tree_state bytes leaf_ind & bytes)
+let commit #bytes #cb #leaf_ind st #li p excluded_leaves group_context =
+  let un_added_tree = un_add st.tree excluded_leaves in
+  treekem_invariant_un_add st.tree excluded_leaves;
+  treekem_priv_invariant_un_add st.tree st.priv excluded_leaves;
+  if not (check_update_path_ciphertexts_lengthes un_added_tree p) then (
+    error "TreeKEM.commit: bad UpdatePath ciphertext lengths"
+  ) else (
+    weaken_path_filtering_ok st.tree p;
+    path_filtering_weak_ok_un_add st.tree p excluded_leaves;
+    let? (path_secret, least_common_ancestor_level) = get_path_secret un_added_tree st.priv p group_context in
+    let new_tree = tree_apply_path st.tree p in
+    let? (new_priv, root_secret) = path_apply_path new_tree st.priv path_secret least_common_ancestor_level in
+    treekem_invariant_apply_path st.tree p;
+    treekem_priv_invariant_apply_path st.tree st.priv p path_secret least_common_ancestor_level;
+    return ({ st with
+      tree = new_tree;
+      priv = new_priv;
+    }, root_secret)
+  )
+
+(*** Create Commit ***)
+
+val prepare_create_commit_entropy_lengths:
+  bytes:Type0 -> {|crypto_bytes bytes|} ->
+  list nat
+let prepare_create_commit_entropy_lengths bytes #cb =
+  [hpke_private_key_length #bytes; kdf_length #bytes]
+
+type pending_commit (#bytes:Type0) {|crypto_bytes bytes|} (#leaf_ind:nat) (st:treekem_tree_state bytes leaf_ind) = {
+  path_secrets: path_secrets:path_secrets bytes st.levels 0 leaf_ind{path_filtering_ok st.tree path_secrets /\ forget_path_secrets path_secrets == generate_forgotten_path_secrets st.tree leaf_ind};
+  commit_secret: bytes;
+}
+
+val prepare_create_commit:
+  #bytes:Type0 -> {|crypto_bytes bytes|} -> #leaf_ind:nat ->
+  st:treekem_tree_state bytes leaf_ind ->
+  randomness bytes (prepare_create_commit_entropy_lengths bytes) ->
+  result (pending_commit st & pre_pathkem bytes st.levels 0 leaf_ind)
+let prepare_create_commit #bytes #cb #leaf_ind st rand =
+  let leaf_sk, rand = dest_randomness rand in
+  let path_secret_0, rand = dest_randomness rand in
+  let? (path_secrets, commit_secret) = generate_path_secrets st.tree leaf_sk path_secret_0 leaf_ind in
+  let? pre_upd_path = path_secrets_to_pre_pathkem path_secrets in
+  path_filtering_ok_generate_path_secrets st.tree leaf_sk path_secret_0 leaf_ind;
+  return ({
+    path_secrets;
+    commit_secret;
+  }, pre_upd_path)
+
+val finalize_create_commit_entropy_lengths:
+  #bytes:Type0 -> {|crypto_bytes bytes|} -> #leaf_ind:nat ->
+  st:treekem_tree_state bytes leaf_ind -> list nat ->
+  list nat
+let finalize_create_commit_entropy_lengths #bytes #cb #leaf_ind st added_leaves =
+  treekem_invariant_un_add st.tree added_leaves;
+  let path_secrets = generate_forgotten_path_secrets st.tree leaf_ind in
+  encrypt_path_secrets_entropy_lengths (un_add st.tree added_leaves) path_secrets
+
+type create_commit_result (#bytes:Type0) {|crypto_bytes bytes|} (#leaf_ind:nat) (st:treekem_tree_state bytes leaf_ind) = {
+  new_state: treekem_tree_state bytes leaf_ind;
+  update_path: update_path:pathkem bytes st.levels 0 leaf_ind{path_filtering_ok st.tree update_path};
+  commit_secret: bytes;
+  added_leaves_path_secrets: list bytes;
+}
+
+val finalize_create_commit:
+  #bytes:Type0 -> {|crypto_bytes bytes|} -> #leaf_ind:nat ->
+  #st:treekem_tree_state bytes leaf_ind ->
+  pending_commit st ->
+  added_leaves:list nat -> group_context_nt bytes ->
+  randomness bytes (finalize_create_commit_entropy_lengths st added_leaves) ->
+  result (create_commit_result st)
+let finalize_create_commit #bytes #cb #leaf_ind #st pending added_leaves group_context randomness =
+  treekem_invariant_un_add st.tree added_leaves;
+  let? (update_path, new_priv) = encrypt_path_secrets (un_add st.tree added_leaves) pending.path_secrets group_context randomness in
+  let? added_leaves_path_secrets = get_path_secret_of_added_leaves pending.path_secrets added_leaves in
+  let new_tree = tree_apply_path st.tree update_path in
+  path_filtering_ok_encrypt_path_secrets st.tree (un_add st.tree added_leaves) pending.path_secrets group_context randomness;
+  treekem_invariant_apply_path st.tree update_path;
+  treekem_priv_invariant_encrypt_path_secrets st.tree (un_add st.tree added_leaves) pending.path_secrets group_context randomness;
+  return ({
+    new_state = { st with
+      tree = new_tree;
+      priv = new_priv;
+    };
+    update_path;
+    commit_secret = pending.commit_secret;
+    added_leaves_path_secrets;
+  })
